theories/Alpha/RenameApart_Alpha.v
@@ -4,19 +4,20 @@ Require Import LabelsDefined PairwiseDisjoint RenameApart.
 
 Set Implicit Arguments.
 
-Lemma rename_apart_alpha' fresh G ϱ ϱ' s
-  : lookup_set ϱ (freeVars s) ⊆ G
+Lemma rename_apart_alpha' {Fi} (FG:FreshGen Fi) (FGS:FreshGenSpec FG) fi ϱ ϱ' s
+  : lookup_set ϱ (freeVars s) ⊆ domain _ fi
   -> inverse_on (freeVars s) ϱ ϱ'
-  -> alpha ϱ' ϱ (snd (renameApart' fresh ϱ G s)) s.
+  -> alpha ϱ' ϱ (snd (renameApart' FG fi ϱ s)) s.
 Proof.
-  revert G ϱ ϱ'.
-  sind s; destruct s; simpl; intros; repeat let_pair_case_eq; subst;
+  revert fi ϱ ϱ'.
+  induction s using stmt_ind'; simpl; intros; repeat let_pair_case_eq; subst;
   simpl in * |- *; eauto using alpha.
 
   - econstructor. eapply alpha_exp_sym. eapply alpha_exp_rename_injective.
     eapply inverse_on_incl; try eassumption. eauto with cset.
-    eapply IH; eauto.
-    + rewrite <- H at 3. rewrite lookup_set_update_in_union; eauto.
+    eapply IHs; eauto.
+    + rewrite fresh_domain_spec; eauto.
+      rewrite <- H. rewrite lookup_set_update_in_union; eauto.
       rewrite <- lookup_set_union_incl; eauto; try reflexivity.
       cset_tac.
     + eapply inverse_on_update_inverse. intuition.
@@ -24,17 +25,18 @@ Proof.
       assert (lookup_set ϱ (freeVars s \ {{x}}) ⊆
                          lookup_set ϱ ((freeVars s \ {{x}}) ∪ Exp.freeVars e)).
       rewrite lookup_set_union; cset_tac; intuition.
-      rewrite H1, H. eauto.
+      rewrite H1, H. eapply fresh_spec; eauto.
   - econstructor; eauto.
     + eapply alpha_op_sym. eapply alpha_op_rename_injective.
       eapply inverse_on_incl; try eassumption. eapply incl_right.
-    + eapply IH; eauto.
+    + eapply IHs1; eauto.
       * eapply Subset_trans; try eassumption. eapply lookup_set_incl; [intuition|].
         rewrite union_assoc, union_comm. eapply incl_right.
       * eapply inverse_on_incl; try eassumption.
         rewrite union_assoc, union_comm. eapply incl_right.
-    + eapply IH; eauto.
-      * rewrite <- H at 1. repeat rewrite lookup_set_union; cset_tac; intuition.
+    + eapply IHs2; eauto.
+      * rewrite renameApart'_domain; eauto.
+        rewrite <- H. repeat rewrite lookup_set_union; cset_tac; intuition.
       * eapply inverse_on_incl; try eassumption.
         cset_tac; intuition.
   - econstructor. rewrite map_length; eauto.
@@ -48,46 +50,41 @@ Proof.
     eapply inverse_on_incl; try eassumption. reflexivity.
   - econstructor.
     + rewrite rev_length, renameApartF_length; eauto.
-    + intros. eapply get_rev in H1.
-      rewrite renameApartF_length in H1.
-      edestruct get_fst_renameApartF as [? [? [? ]]]; dcr; eauto.
-      exploit (get_range H2).
-      orewrite (length F - S (length F - S n) = n) in H4. get_functional; subst.
-      eauto.
-    + intros.
-      eapply get_rev in H1.
-      rewrite renameApartF_length in H1; eauto.
-      edestruct get_fst_renameApartF as [? [? [? ]]]; dcr; eauto.
-      exploit (get_range H2).
-      orewrite (length F - S (length F - S n) = n) in H4. get_functional; subst.
-      setoid_rewrite H6.
-      erewrite renameApart'_agree; eauto. eapply IH; eauto.
-      * rewrite lookup_set_update_with_list_in_union_length; eauto.
-        eapply union_subset_3; eauto.
-        rewrite <- H5.
-        rewrite <- H.
-        eapply lookup_set_incl; eauto.
-        eapply incl_union_left.
-        eapply incl_list_union. eapply map_get_1; eauto. reflexivity.
-      * eapply inverse_on_update_fresh; eauto.
-        eapply inverse_on_incl; try eassumption. eauto.
-        eapply incl_union_left.
-        eapply incl_list_union. eapply map_get_1; eauto. reflexivity.
-        symmetry. eapply disj_1_incl; eauto.
-        rewrite <- H. eapply lookup_set_incl; eauto.
-        eapply incl_union_left.
-        eapply incl_list_union. eapply map_get_1; eauto. reflexivity.
-      * symmetry. eapply agree_on_incl; eauto with cset.
-    + eapply IH; eauto.
-      * rewrite <- H at 1.
+    + intros. inv_get. len_simpl. inv_get. rewrite fresh_list_len; eauto.
+    + intros. inv_get; len_simpl. inv_get.
+      * eapply H; eauto.
+        -- rewrite lookup_set_update_with_list_in_union_length; eauto.
+           rewrite fresh_list_domain_spec; eauto.
+           rewrite union_comm. eapply incl_union_lr; eauto.
+           rewrite <- domain_incl_renameApartFRight; eauto.
+           rewrite <- H0.
+           eapply lookup_set_incl; eauto.
+           eapply incl_union_left.
+           eapply incl_list_union. eapply map_get_1; eauto. reflexivity.
+           rewrite fresh_list_len; eauto.
+        -- eapply inverse_on_update_fresh; eauto.
+           eapply inverse_on_incl; try eassumption. eauto.
+           eapply incl_union_left.
+           eapply incl_list_union. eapply map_get_1; eauto. reflexivity.
+           eapply fresh_list_nodup; eauto.
+           rewrite fresh_list_len; eauto.
+           symmetry. eapply disj_1_incl; eauto.
+           eapply fresh_list_disj; eauto.
+           rewrite <- domain_incl_renameApartFRight; eauto.
+           rewrite <- H0. eapply lookup_set_incl; eauto.
+           eapply incl_union_left.
+           eapply incl_list_union. eapply map_get_1; eauto. reflexivity.
+    + eapply IHs; eauto.
+      * rewrite <- domain_incl_renameApartF; eauto.
+        rewrite <- H0 at 1.
         rewrite lookup_set_union; eauto with cset.
       * eapply inverse_on_incl; try eassumption. eauto.
 Qed.
 
-Lemma rename_apart_alpha fresh s
-  : alpha id id (rename_apart fresh s) s.
+Lemma rename_apart_alpha {Fi} (FG:FreshGen Fi) (FGS:FreshGenSpec FG) fi s
+  : alpha id id (rename_apart FG (domain_add FG fi (freeVars s)) s) s.
 Proof.
-  eapply rename_apart_alpha'.
-  + eapply lookup_set_on_id; reflexivity.
+  eapply rename_apart_alpha'; eauto.
+  + eapply lookup_set_on_id. rewrite domain_add_spec; eauto with cset.
   + eapply inverse_on_id.
 Qed.
