theories/Alpha/RenamedApartAnn.v
@@ -1,0 +1,325 @@
+Require Import CSet Util Map.
+Require Import Env IL Alpha StableFresh Annotation RenamedApart SetOperations.
+Require Import LabelsDefined PairwiseDisjoint AppExpFree.
+Require Import Infra.PartialOrder CSetPartialOrder AnnotationLattice.
+
+Require Import RenamedApart.
+
+Set Implicit Arguments.
+
+Definition renamedApartAnnF (renamedApartAnn:stmt -> set var -> ann (set var * set var)) G
+           := fold_left (fun anFG (Zs:params*stmt) =>
+                        let ans := renamedApartAnn (snd Zs) (G ∪ of_list (fst Zs)) in
+                        (ans::fst anFG, snd anFG ∪ (of_list (fst Zs) ∪ snd (getAnn ans)))).
+
+Fixpoint renamedApartAnn (s:stmt) (G:set var) : ann (set var * set var) :=
+  match s with
+    | stmtLet x e s =>
+      let an := renamedApartAnn s {x; G} in
+      ann1 (G, {x; snd (getAnn an) }) an
+    | stmtIf e s t =>
+      let ans := renamedApartAnn s G in
+      let ant := renamedApartAnn t G in
+      ann2 (G, snd (getAnn ans) ∪ snd (getAnn ant)) ans ant
+    | stmtReturn e =>
+      ann0 (G, ∅)
+    | stmtApp f Y =>
+      ann0 (G, ∅)
+    | stmtFun F t =>
+      let (ans, G') := renamedApartAnnF renamedApartAnn G F (nil, {}) in
+      let ant := renamedApartAnn t G in
+      annF (G, G' ∪ (snd (getAnn ant))) (rev ans) ant
+  end.
+
+Lemma fst_renamedApartAnn s G
+ : fst (getAnn (renamedApartAnn s G)) = G.
+Proof.
+  sind s; destruct s; eauto.
+  - simpl. let_pair_case_eq. simpl; eauto.
+Qed.
+
+Lemma snd_renamedApartAnnF' F L G G'
+: (forall n Zs G',
+     get F n Zs ->
+     snd (getAnn (renamedApartAnn (snd Zs) G')) = definedVars (snd Zs))
+  -> snd (renamedApartAnnF renamedApartAnn G F (L, G')) =
+    fold_left union (defVarsZs definedVars ⊝ F) G'.
+Proof.
+  intros.
+  general induction F; intros; simpl; eauto.
+  - rewrite IHF; eauto using get.
+    erewrite H; eauto using get.
+Qed.
+
+Lemma snd_renamedApartAnnF_nil' G F
+: (forall n Zs, get F n Zs -> forall G, snd (getAnn (renamedApartAnn (snd Zs) G)) = definedVars (snd Zs))
+  -> snd (renamedApartAnnF renamedApartAnn G F (nil, {})) = definedVarsF definedVars F.
+Proof.
+  intros. rewrite snd_renamedApartAnnF'; eauto.
+Qed.
+
+Lemma get_fst_renamedApartAnnF' G F n ans L G'
+:  get (fst (renamedApartAnnF renamedApartAnn G F (L, G'))) n ans
+   -> (get L (n - ❬F❭) ans /\ n >= ❬F❭ ) \/
+     (n < ❬F❭ /\ exists Zs, get F (❬F❭ - S n) Zs
+                      /\ ans = renamedApartAnn (snd Zs) (G ∪ of_list (fst Zs))).
+Proof.
+  general induction F; simpl in * |- *;[ isabsurd |].
+  - left. split; eauto. orewrite (n - 0 = n). eauto. omega.
+  - eapply IHF in H as [[? ?]|[? [? [? ?]]]]; simpl in *.
+    + inv H; eauto using get.
+      * right.
+        assert (n = ❬F❭) by omega; subst.
+        rewrite <- H4 in *.
+        split; eauto. eauto using get.
+      * left. orewrite (n - S ❬F❭ = n0). split; eauto. omega.
+    + subst. right. split. omega.
+      eexists x; split; eauto using get.
+      orewrite (❬F❭ - n = S (❬F❭ - S n)). econstructor; eauto.
+Qed.
+
+Lemma get_fst_renamedApartAnnF G F n ans G'
+:  get (fst (renamedApartAnnF renamedApartAnn G F (nil, G'))) n ans
+   -> exists Zs, get F (❬F❭ - S n) Zs
+           /\ ans = renamedApartAnn (snd Zs) (G ∪ of_list (fst Zs)).
+Proof.
+  intros. eapply get_fst_renamedApartAnnF' in H; destruct H; isabsurd.
+  dcr; eauto.
+Qed.
+
+Lemma length_fst_renamedApartAnnF' G G' F L
+: length (fst (renamedApartAnnF renamedApartAnn G F (L, G')))
+  = ❬L❭ + length F.
+Proof.
+  general induction F; simpl; eauto.
+  rewrite IHF; eauto; simpl. omega.
+Qed.
+
+Lemma length_fst_renamedApartAnnF G G' F
+: length (fst (renamedApartAnnF renamedApartAnn G F (nil, G'))) = length F.
+Proof.
+  rewrite length_fst_renamedApartAnnF'. reflexivity.
+Qed.
+
+Smpl Add
+      match goal with
+      | [ H :  get (fst (renamedApartAnnF renamedApartAnn ?G (rev ?F) (nil, {})))
+                   (❬fst (renamedApartAnnF renamedApartAnn ?G (rev ?F) (nil, {}))❭ - S ?n) ?b |- _ ] =>
+        let GET := fresh "Get" in
+        eapply get_fst_renamedApartAnnF in H as [? [GET ?]]; subst;
+          rewrite length_fst_renamedApartAnnF in GET;
+          eapply get_rev in GET;
+          rewrite rev_length in GET
+      | [ H :  get (fst (renamedApartAnnF renamedApartAnn ?G ?F (nil, {})))
+                   (❬fst (renamedApartAnnF renamedApartAnn ?G ?F (nil, {}))❭ - S ?n) ?b |- _ ] =>
+        let GET := fresh "Get" in
+        eapply get_fst_renamedApartAnnF in H as [? [GET ?]]; subst;
+          rewrite length_fst_renamedApartAnnF in GET
+      end : inv_get.
+
+Lemma get_index_rev k n
+  : k - S (k - S (k - S n)) = k - S n.
+  omega.
+Qed.
+
+Smpl Add
+     match goal with
+       [ H : get _ (?k - S (?k - S (?k - S ?n))) _ |- _ ] =>
+       rewrite (get_index_rev k n) in H
+     end : inv_get.
+
+Lemma snd_renamedApartAnn s G
+: snd (getAnn (renamedApartAnn s G)) = definedVars s.
+Proof.
+  revert G.
+  induction s using stmt_ind'; simpl; intros; repeat let_pair_case_eq; simpl; eauto; subst.
+  - rewrite (IHs); eauto.
+  - rewrite (IHs1); eauto. rewrite (IHs2); eauto.
+  - rewrite (IHs); eauto.
+    rewrite snd_renamedApartAnnF_nil'; eauto.
+Qed.
+
+Lemma snd_renamedApartAnnF F L G G'
+  : snd (renamedApartAnnF renamedApartAnn G F (L, G')) =
+    fold_left union (defVarsZs definedVars ⊝ F) G'.
+Proof.
+  eapply snd_renamedApartAnnF'; eauto using snd_renamedApartAnn.
+Qed.
+
+
+Lemma renamedApartAnn_decomp s G
+: pe (getAnn (renamedApartAnn s G)) (G, snd (getAnn (renamedApartAnn s G))).
+Proof.
+  destruct s; simpl; try reflexivity.
+  - let_pair_case_eq; simpl_pair_eqs; subst; simpl; eauto.
+Qed.
+
+
+Ltac renamedApart_len_simpl :=
+  match goal with
+  | [ H : context [ fst (renamedApartAnnF _ ?G ?F (nil, ?G'))] |- _ ] =>
+    rewrite (length_fst_renamedApartAnnF G G' F) in H
+  | [ |- context [ fst (renamedApartAnnF _ ?G ?F (nil, ?G'))] ] =>
+    rewrite (length_fst_renamedApartAnnF G G' F)
+  end.
+
+Smpl Add renamedApart_len_simpl : len.
+
+Lemma add_minus_eq X `{OrderedType X} G1 G2 x G'
+  :  G1 [=] G2 \ G' -> x ∉ G' -> {x; G1} [=] {x; G2} \ G'.
+Proof.
+  intros. rewrite H0; clear H0. cset_tac.
+Qed.
+
+Hint Resolve add_minus_eq : cset.
+
+(*
+Local Hint Extern 10 =>
+match goal with
+| [ |- context [ snd (getAnn (renamedApartAnn ?s ?G))] ] => setoid_rewrite snd_renamedApartAnn
+| [ |- context [ snd (renamedApartAnnF renamedApartAnn ?G (nil, _) ?s) ] ]
+  => setoid_rewrite snd_renamedApartAnnF
+end : ann.
+
+Lemma ann_R_pe_notOccur G1 G2 G' s
+:  disj (occurVars s) G'
+   -> G1 [=] G2 \ G'
+   -> ann_R (@pe var _)
+           (renamedApartAnn s G1)
+           (mapAnn (pminus G') (renamedApartAnn s G2)).
+Proof.
+  revert G1 G2 G'.
+  sind s; destruct s; intros; simpl in * |- *; eauto using pe, ann_R with cset;
+  try now (econstructor; reflexivity).
+  - econstructor; eauto 20 with pe ann cset.
+  - econstructor; eauto with cset pe ann.
+  - econstructor; eauto with cset pe ann.
+  - econstructor; eauto with cset pe ann.
+  - intros.
+    repeat let_pair_case_eq; subst; simpl.
+    econstructor; eauto 20 with cset pe ann.
+    + rewrite List.map_length; eauto.
+      repeat rewrite length_fst_renamedApartAnnF; eauto.
+    + intros.
+      inv_map H2.
+      edestruct get_fst_renamedApartAnnF as [? [? ?]]; dcr; eauto. subst.
+      edestruct get_fst_renamedApartAnnF as [? [? ?]]; dcr; try eapply H1; eauto. subst.
+      get_functional; subst.
+      eapply IH; eauto.
+      * eapply disj_1_incl; eauto.
+        eapply incl_union_left.
+        eapply incl_list_union; eauto using map_get_1 with cset.
+      * repeat rewrite minus_dist_union.
+        rewrite H0.
+        eapply union_eq_decomp; eauto.
+        eapply disj_eq_minus; eauto.
+        eapply disj_1_incl; eauto.
+        eapply incl_union_left.
+        eapply incl_list_union. eapply map_get_1; eauto.
+        eapply incl_right.
+Qed.
+ *)
+
+
+Lemma fst_renamedApartAnnF_swap G G' F L
+  : fst (renamedApartAnnF renamedApartAnn G F (L, G'))
+    = fst (renamedApartAnnF renamedApartAnn G F (nil, G')) ++ L.
+Proof.
+  general induction F; simpl; eauto.
+  setoid_rewrite IHF at 1.
+  setoid_rewrite IHF at 2.
+  rewrite <- !app_assoc.
+  rewrite <- cons_app. reflexivity.
+Qed.
+
+Lemma fst_renamedApartAnnF_eq G G1 G2 F L
+  : fst (renamedApartAnnF renamedApartAnn G F (L, G1))
+    = fst (renamedApartAnnF renamedApartAnn G F (L, G2)).
+Proof.
+  general induction F; simpl; eauto.
+Qed.
+
+Ltac renamedApartAnnF_swap_normal :=
+  repeat match goal with
+           [ |- context [ renamedApartAnnF ?f ?G ?F (?L, ?G') ] ] =>
+           match L with
+           | nil => fail 1
+           | _ => rewrite (@fst_renamedApartAnnF_swap G G' F L)
+           end
+         end.
+
+Lemma fst_renamedApartAnnF_app G F F' L G'
+  : fst (renamedApartAnnF renamedApartAnn G (F ++ F') (L, G'))
+    = fst (renamedApartAnnF renamedApartAnn G F' (nil, snd ((renamedApartAnnF renamedApartAnn G F (nil, G')))))
+          ++ fst (renamedApartAnnF renamedApartAnn G F (L, G')).
+Proof.
+  general induction F; simpl; eauto.
+  - rewrite fst_renamedApartAnnF_swap. reflexivity.
+  - rewrite IHF.
+    rewrite !snd_renamedApartAnnF; eauto.
+Qed.
+
+Lemma fst_renamedApartAnnF_rev G F
+  : fst (renamedApartAnnF renamedApartAnn G (rev F) (nil, G))
+    = rev (fst (renamedApartAnnF renamedApartAnn G F (nil, G))).
+Proof.
+  induction F; simpl; eauto.
+  renamedApartAnnF_swap_normal.
+  rewrite !fst_renamedApartAnnF_app; simpl.
+  rewrite rev_app_distr; simpl.
+  f_equal. rewrite IHF.
+  erewrite fst_renamedApartAnnF_eq; eauto.
+Qed.
+
+Lemma poEq_add X `{OrderedType X} (x y:X) s t
+  : _eq x y
+    -> poEq s t
+    -> poEq {x; s} {y; t}.
+Proof.
+  intros. rewrite H0. rewrite H1. reflexivity.
+Qed.
+
+Hint Resolve poEq_add.
+
+Lemma poEq_union X `{OrderedType X} s s' t t'
+  : poEq s t
+    -> poEq s' t'
+    -> poEq (s ∪ s') (t ∪ t').
+Proof.
+  intros. rewrite H0. rewrite H1. reflexivity.
+Qed.
+
+Hint Resolve poEq_union.
+
+Lemma poEq_rev X `{PartialOrder X} L L'
+  : poEq L L'
+    -> poEq (rev L) (rev L').
+Proof.
+  intros. general induction H0; simpl; eauto.
+
+Qed.
+
+Hint Resolve poEq_rev.
+
+Lemma renamedApartAnnF_ext G G' F L1 L2 G1 G2
+  (IH: forall (n : nat) (Zs : params * stmt),
+      get F n Zs ->
+      forall G G' : ⦃nat⦄,
+      G ≣ G' -> renamedApartAnn (snd Zs) G ≣ renamedApartAnn (snd Zs) G')
+  : G ≣ G'
+    -> L1 ≣ L2
+    -> G1 ≣ G2
+    -> renamedApartAnnF renamedApartAnn G F (L1, G1) ≣
+                     renamedApartAnnF renamedApartAnn G' F (L2, G2).
+Proof.
+  general induction F; simpl; eauto 200 using get.
+Qed.
+
+Lemma renamedApartAnn_ext G G' s
+  : poEq G G'
+    -> poEq (renamedApartAnn s G) (renamedApartAnn s G').
+Proof.
+  revert G G'.
+  induction s using stmt_ind'; intros; simpl;
+    repeat let_pair_case_eq; subst; eauto 200 using renamedApartAnnF_ext.
+Qed.
